Remove modifyS as it is was dead code.
This also means modifyS'' -> modifyS'
and modifyS' -> modifyS

theories/program_logic/delaystate.v
@@ -195,11 +195,8 @@ refine (λ a, iter_state_delay
 Defined.
 
 (*Next up implement the state operations! *)
-Definition modifyS' {A ST} (f: ST -> ST * A): state_delay ST A :=
+Definition modifyS {A ST} (f: ST -> ST * A): state_delay ST A :=
   State $ λ s, Answer $ Some $ f s.
-
-Definition modifyS {ST} (f: ST -> ST): state_delay ST () :=
-  modifyS' $ λ st, (f st, tt).
 
 Definition getS {ST}: state_delay ST ST :=
   State $ λ st, Answer $ Some $ (st, st).
@@ -216,17 +213,17 @@ Definition ret_fail {ST A} (m: option A): state_delay ST A :=
   |None => fail
   end.
 
- Definition modifyS'' {A} (n: nat) (f: gmap nat A -> gmap nat A): state_delay (gmap nat A) () :=
+ Definition modifyS' {A} (n: nat) (f: gmap nat A -> gmap nat A): state_delay (gmap nat A) () :=
     State $ λ st, if decide (is_Some (st !! n)) then Answer $ Some (f st, tt) else  Answer $ None.
 
 Definition get {A} (n: nat): state_delay (gmap nat A) A :=
   getS ≫= λ st, ret_fail $ lookup n st.
 
   Definition put {A} (n: nat) (x : A) : state_delay (gmap nat A) unit :=
-  modifyS'' n  <[n := x]>.
+  modifyS' n  <[n := x]>.
 
 Definition alloc {A} (v: A) : state_delay (gmap nat A) nat :=
-  modifyS' $ λ st, 
+  modifyS $ λ st, 
               let fresh := fresh $ dom (gset nat) st
               in (<[fresh := v]> st, fresh). 
 
@@ -234,7 +231,7 @@ Definition alloc {A} (v: A) : state_delay (gmap nat A) nat :=
   modifyS $ delete n. *)
 
 Definition free {A} (n: nat): state_delay (gmap nat A) unit :=
-  modifyS'' n (delete n).
+  modifyS' n (delete n).
 
 Fixpoint eval_delay {A} (n: nat) (ma: delay A): option A :=
   match n with
