theories/program_logic/itreewp.v
@@ -979,7 +979,8 @@ End adequacy.
      let's lift that.
      Now I need to get it in a big op
 *)
-Lemma adequacy {V Σ} {cmp: EqDecision V} `{!inG Σ (heapR V)} `{!invGpreS Σ} {R} (φ: R -> Prop) (n: nat)
+Lemma adequacy {V Σ} {cmp: EqDecision V} `{!inG Σ (heapR V)} `{!invGpreS Σ} {R}
+  (φ: R -> Prop) (n: nat)
   (SI: gmap nat V -> iProp Σ)
   (s: scheduler V R)
   (e: expr V R)
